src/Util.fsti
@@ -2,7 +2,7 @@ module Util
 
 open FStar.List
 
-val range : n:nat -> list (m:nat{m < n})
+val range : n:pos -> list (m:nat{m < n})
 
 val lemma_range_complete : n:nat -> Lemma
 	(forall m. m < n <==> mem m (range n))
