Makefile
@@ -1,3 +1,7 @@
+FSTAR=fstar.exe
+FSTAR_OPTS=--include src --log_queries --record_hints
+
 all:
-	fstar.exe src/QuickCodes.fst --include src --log_queries --record_hints
-	fstar.exe src/Regs.fst --include src --log_queries --record_hints
+	$(FSTAR) src/QuickCodes.fst $(FSTAR_OPTS)
+	$(FSTAR) src/Regs.fst $(FSTAR_OPTS)
+	$(FSTAR) src/
